src/BinEncoders/Env/Common/Specs.v
@@ -4,14 +4,20 @@ Require Export
 Set Implicit Arguments.
 
 Section Specifications.
-  Variable A B C E E' Z : Type.
+  Variable A B E E' : Type.
+
+  Class Transformer :=
+    { transform : B -> B -> B;
+      transform_id : B;
+      transform_id_pf : forall l, transform transform_id l = l;
+      transform_assoc : forall l m n, transform l (transform m n) = transform (transform l m) n }.
 
   Definition encode_decode_correct
              (envequiv  : E -> E' -> Prop)
-             (transform : B -> C -> Z)
+             (transformer : Transformer)
              (predicate : A -> Prop)
              (encode : A -> E -> B * E)
-             (decode :  Z -> E' -> A * C * E') :=
+             (decode :  B -> E' -> A * B * E') :=
     forall env env' xenv xenv' data data' bin ext ext',
       envequiv env env' ->
       predicate data ->
@@ -21,9 +27,9 @@ Section Specifications.
 
   Class decoder
         (envequiv  : E -> E' -> Prop)
-        (transform : B -> C -> Z)
+        (transformer : Transformer)
         (predicate : A -> Prop)
         (encode : A -> E -> B * E) :=
-    { decode : Z -> E' -> A * C * E';
-      decode_correct : encode_decode_correct envequiv transform predicate encode decode }.
+    { decode : B -> E' -> A * B * E';
+      decode_correct : encode_decode_correct envequiv transformer predicate encode decode }.
 End Specifications.
